src/impl/TLS13.Connection.fsti
@@ -21,6 +21,9 @@ val connection_exactly: connection -> ST.state_ref -> S.conn_state -> CL.connect
 
 val is_connection: connection -> ST.state_ref -> S.conn_state -> slprop
 
+noextract
+val connection_hostname: connection -> T.hostname
+
 ghost
 fn reveal_connection_view (c: connection)
   requires is_connection c 'st 's
@@ -40,7 +43,8 @@ fn client_new
   returns c: connection
   ensures exists* st.
           pts_to hostname 'hostname_bytes **
-          connection_exactly c st S.initial CL.empty_connection_view
+          connection_exactly c st S.initial CL.empty_connection_view **
+          pure (connection_hostname c == Ghost.reveal 'hostname_bytes)
 
 fn client_free (c: connection)
   requires connection_exactly c 'st 's 'view
@@ -54,8 +58,8 @@ fn client_connect (c: connection) (ch: IO.channel)
   ensures exists* s' view1. connection_exactly c 'st s' view1 **
           IO.is_channel ch **
           pure (CL.connection_view_single_step 'view0 view1 /\
-                (exists server_name resp.
-                   CL.step 'view0 (CL.request_no_network_in (CL.OpStart server_name)) view1 resp /\
+                (exists resp.
+                   CL.step 'view0 (CL.request_no_network_in (CL.OpStart (connection_hostname c))) view1 resp /\
                    (ok ==> resp.CL.status == CL.HandshakeComplete) /\
                    (not ok ==> resp.CL.status == CL.Failed T.IoError)) /\
                 (ok ==> s'.S.phase == S.ApplicationData) /\
